WIP: Fix LDRF-PF proof

src/ldrfpf/TimeTraced.v
@@ -40,9 +40,9 @@ Inductive times_configuration_step_strong (times: Loc.t -> Time.t -> Prop)
     (SILENT: List.Forall (fun the => ThreadEvent.get_machine_event (snd the) = MachineEvent.silent) tr')
     (STEP: Thread.step pf e e2 (Thread.mk _ st3 lc3 sc3 memory3))
     (TR: tr = tr'++[((Thread.local e2), e)])
-    (CONSISTENT: forall (EVENT: e <> ThreadEvent.failure),
+    (CONSISTENT: forall (EVENT: ThreadEvent.get_machine_event e <> MachineEvent.failure),
         pf_consistent_super_strong (Thread.mk _ st3 lc3 sc3 memory3) tr_cert times)
-    (CERTBOT: e = ThreadEvent.failure \/ (exists se, e = ThreadEvent.syscall se) -> tr_cert = [])
+    (CERTBOT: ThreadEvent.get_machine_event e = MachineEvent.failure \/ (exists se, e = ThreadEvent.syscall se) -> tr_cert = [])
     (CERTBOTNIL: (Local.promises lc3) = Memory.bot -> tr_cert = [])
     (TIMES: List.Forall (fun thte => wf_time_evt times (snd thte)) tr)
   :
@@ -61,9 +61,9 @@ Inductive times_configuration_step (times: Loc.t -> Time.t -> Prop)
     (SILENT: List.Forall (fun the => ThreadEvent.get_machine_event (snd the) = MachineEvent.silent) tr')
     (STEP: Thread.step pf e e2 (Thread.mk _ st3 lc3 sc3 memory3))
     (TR: tr = tr'++[((Thread.local e2), e)])
-    (CONSISTENT: forall (EVENT: e <> ThreadEvent.failure),
+    (CONSISTENT: forall (EVENT: ThreadEvent.get_machine_event e <> MachineEvent.failure),
         pf_consistent_super_strong (Thread.mk _ st3 lc3 sc3 memory3) tr_cert times)
-    (CERTBOT: e = ThreadEvent.failure \/ (exists se, e = ThreadEvent.syscall se) -> tr_cert = [])
+    (CERTBOT: ThreadEvent.get_machine_event e = MachineEvent.failure \/ (exists se, e = ThreadEvent.syscall se) -> tr_cert = [])
     (TIMES: List.Forall (fun thte => wf_time_evt times (snd thte)) tr)
   :
     times_configuration_step
@@ -92,12 +92,12 @@ Lemma times_configuration_step_configuration_step times tr tr_cert e tid c1 c2
     Configuration.step e tid c1 c2.
 Proof.
   inv STEP. eapply Trace.silent_steps_tau_steps in STEPS; eauto.
-  destruct (classic (e0 = ThreadEvent.failure)).
-  { subst. econs; eauto. }
+  destruct (classic (ThreadEvent.get_machine_event e0 = MachineEvent.failure)).
+  { econs; eauto. ss. }
   { inv WF. exploit Thread.rtc_tau_step_future; ss; eauto.
     { eapply WF0; eauto. } i. des.
     exploit Thread.step_future; ss; eauto. ss. i. des.
-    econs 2; eauto. eapply pf_consistent_super_strong_consistent; eauto.
+    econs; eauto. i. eapply pf_consistent_super_strong_consistent; eauto.
   }
 Qed.
 
@@ -175,65 +175,85 @@ Lemma times_configuration_step_exists c0 c1 tid e
       (WF: Configuration.wf c0)
   :
     exists times tr tr_cert,
-      (<<STEP: @times_configuration_step_strong times tr tr_cert e tid c0 c1>>) /\
+      ((<<STEP: @times_configuration_step_strong times tr tr_cert e tid c0 c1>>) \/
+       exists c1',
+         (<<STEP: @times_configuration_step_strong times tr tr_cert MachineEvent.failure tid c0 c1'>>))
+      /\
       (<<WO: forall loc, well_ordered (times loc)>>).
 Proof.
   inv STEP.
-  { eapply Trace.tau_steps_silent_steps in STEPS. des.
+  destruct (classic (Thread.steps_failure (Thread.mk _ st1 lc1 c0.(Configuration.sc) c0.(Configuration.memory)))) as [FAILURE|NFAILURE].
+  { clear STEPS STEP0 EVENT. red in FAILURE. des. destruct e3.
+    eapply Trace.tau_steps_silent_steps in STEPS. des.
     hexploit (trace_times_list_exists tr). i. des.
     hexploit step_times_list_exists; eauto. i. des.
-    replace MachineEvent.failure with (ThreadEvent.get_machine_event ThreadEvent.failure); auto.
+    replace MachineEvent.failure with (ThreadEvent.get_machine_event e); auto.
     eexists (fun loc ts => List.In ts (times loc ++ times0 loc)), (tr++_), []. splits.
-    { econs; eauto; ss. eapply Forall_app.
+    { right. esplits. econs; eauto; ss. eapply Forall_app.
       { eapply List.Forall_impl; eauto. i. ss. eapply wf_time_evt_mon; eauto.
         i. ss. eapply List.in_or_app; eauto. }
-      { econs; ss. }
+      { econs; ss. eapply wf_time_evt_mon; eauto.
+        i. ss. eapply List.in_or_app; eauto. }
     }
     { i. eapply finite_well_ordered. }
   }
-  { eapply Trace.tau_steps_silent_steps in STEPS. des.
-    hexploit (trace_times_list_exists tr). i. des.
-    hexploit step_times_list_exists; eauto. i. des.
-    hexploit CONSISTENT; ss.
-    dup WF. inv WF. exploit Trace.steps_future; eauto.
-    { ss. eapply WF1; eauto. } i. des. ss.
-    hexploit Thread.step_future; eauto. i. des. ss.
-    eapply consistent_pf_consistent_super_strong in H; eauto. des.
-    destruct (classic ((Local.promises lc3) = Memory.bot)) as [EQBOT|NEQBOT].
-    { des. eexists (certimes \2/ (fun loc ts => List.In ts (times loc ++ times0 loc))), (tr++_), []. splits.
-      { econs; eauto.
-        { i. esplits. eapply promises_bot_certify_nil; eauto. }
-        { eapply Forall_app.
-          { eapply List.Forall_impl; eauto. i. eapply wf_time_evt_mon; try apply H.
-            i. ss. right. eapply List.in_or_app; eauto. }
-          { econs; ss. eapply wf_time_evt_mon; try apply WFTIME0.
-            i. ss. right. eapply List.in_or_app; eauto. }
-        }
+  assert (NORMAL: ThreadEvent.get_machine_event e0 <> MachineEvent.failure).
+  { ii. eapply NFAILURE. red. esplits; eauto.
+    replace pf with true in *; eauto. inv STEP0; inv STEP; ss.
+  }
+  dup STEPS. eapply Trace.tau_steps_silent_steps in STEPS. des.
+  hexploit (trace_times_list_exists tr). i. des.
+  hexploit step_times_list_exists; eauto. i. des.
+  hexploit EVENT; ss.
+  dup WF. inv WF. exploit Trace.steps_future; eauto.
+  { ss. eapply WF1; eauto. } i. des. ss.
+  hexploit Thread.step_future; eauto. i. des. ss.
+  destruct (classic ((Local.promises lc3) = Memory.bot)) as [EQBOT|NEQBOT].
+  { eexists (fun loc ts => List.In ts (times loc ++ times0 loc)), (tr++_), []. splits.
+    { left. econs; eauto.
+      { i. esplits. eapply promises_bot_certify_nil; eauto. }
+      { eapply Forall_app.
+        { eapply List.Forall_impl; eauto. i. eapply wf_time_evt_mon; try apply H0.
+          i. ss. eapply List.in_or_app; eauto. }
+        { econs; ss. eapply wf_time_evt_mon; try apply WFTIME0.
+          i. ss. eapply List.in_or_app; eauto. }
       }
-      { i. eapply join_well_ordered; eauto. eapply finite_well_ordered. }
     }
-    { des. eexists (certimes \2/ (fun loc ts => List.In ts (times loc ++ times0 loc))), (tr++_), tr0. splits.
-      { econs; eauto.
-        { i. esplits. eapply pf_consistent_super_strong_mon; eauto. }
-        { i. des; ss. clarify.
-          inv STEP0; inv STEP. inv LOCAL. inv LOCAL0. ss. exfalso. eauto. }
-        { ii. ss. }
-        { eapply Forall_app.
-          { eapply List.Forall_impl; eauto. i. eapply wf_time_evt_mon; try apply H.
-            i. ss. right. eapply List.in_or_app; eauto. }
-          { econs; ss. eapply wf_time_evt_mon; try apply WFTIME0.
-            i. ss. right. eapply List.in_or_app; eauto. }
-        }
-      }
-      { i. eapply join_well_ordered; eauto. eapply finite_well_ordered. }
+    { i. eapply finite_well_ordered. }
+  }
+  destruct (ThreadEvent.get_machine_event e0) eqn:EQ; ss; cycle 1.
+  { inv STEP0; inv STEP; ss. inv LOCAL; ss.
+    inv LOCAL0; ss. exfalso. eapply NEQBOT; eauto. }
+  eapply consistent_pf_consistent_super_strong in H; eauto. des.
+  { red in FAILURE. des. exfalso. eapply NFAILURE. red. esplits.
+    { etrans.
+      { eapply STEPS0. }
+      econs 2.
+      { econs; [|eapply EQ]. econs; eauto. }
+      { eauto. }
+    }
+    { eauto. }
+    { eauto. }
+  }
+  eexists (certimes \2/ (fun loc ts => List.In ts (times loc ++ times0 loc))), (tr++_), tr0. splits.
+  { left. rewrite <- EQ. econs; eauto.
+    { i. esplits. eapply pf_consistent_super_strong_mon; eauto. }
+    { rewrite EQ. i. des; ss; clarify. }
+    { ii. ss. }
+    { eapply Forall_app.
+      { eapply List.Forall_impl; eauto. i. eapply wf_time_evt_mon; try apply H.
+        i. ss. right. eapply List.in_or_app; eauto. }
+      { econs; ss. eapply wf_time_evt_mon; try apply WFTIME0.
+        i. ss. right. eapply List.in_or_app; eauto. }
     }
   }
+  { i. eapply join_well_ordered; eauto. eapply finite_well_ordered. }
 Qed.
 
 Lemma times_configuration_behavior_configuration_behavior times c
       (WF: Configuration.wf c)
   :
-    behaviors (times_configuration_step_strong_all times) c <1=
+    behaviors (times_configuration_step_strong_all times) c <2=
     behaviors (Configuration.step) c.
 Proof.
   i. ginduction PR; eauto.
@@ -252,14 +272,15 @@ Proof.
     econs 4; eauto. eapply IHPR; eauto.
     eapply Configuration.step_future; eauto.
   }
+  { i. econs 5; eauto. }
 Qed.
 
-Lemma times_configuration_step_same_behaviors c beh
+Lemma times_configuration_step_same_behaviors c f beh
       (WF: Configuration.wf c)
-      (BEH: behaviors Configuration.step c beh)
+      (BEH: behaviors Configuration.step c f beh)
   :
     exists times,
-      (<<BEH: behaviors (times_configuration_step_strong_all times) c beh>>) /\
+      (<<BEH: behaviors (times_configuration_step_strong_all times) c f beh>>) /\
       (<<WO: forall loc, well_ordered (times loc)>>) /\
       (<<INCR: forall nat loc, times loc (incr_time_seq nat)>>) /\
       (<<BOT: forall loc, times loc Time.bot>>)
@@ -278,37 +299,76 @@ Proof.
   { i. exploit IHBEH.
     { eapply Configuration.step_future; eauto. } i. des.
     exploit times_configuration_step_exists; eauto. i. des.
-    exists (times \2/ times0). splits.
-    { econs 2; eauto.
-      { econs. eapply times_configuration_step_strong_mon; eauto. }
-      { eapply le_step_behavior_improve; try apply BEH0.
-        eapply times_configuration_step_strong_all_mon; auto. }
+    { exists (times \2/ times0). splits.
+      { econs 2; eauto.
+        { econs. eapply times_configuration_step_strong_mon; eauto. }
+        { eapply le_step_behavior_improve; try apply BEH0.
+          eapply times_configuration_step_strong_all_mon; auto. }
+      }
+      { i. eapply join_well_ordered; eauto. }
+      { auto. }
+      { auto. }
     }
-    { i. eapply join_well_ordered; eauto. }
-    { auto. }
-    { auto. }
+    { exists (times \2/ times0). splits.
+      { econs 3; eauto.
+        { econs. eapply times_configuration_step_strong_mon; eauto. }
+      }
+      { i. eapply join_well_ordered; eauto. }
+      { auto. }
+      { auto. }
+    }
   }
   { i. exploit times_configuration_step_exists; eauto. i. des.
-    exists (times \2/ (fun loc => incr_times) \2/ (fun _ => eq Time.bot)). splits; eauto.
-    { econs 3; eauto. econs; eauto.
-      eapply times_configuration_step_strong_mon; eauto. }
-    { i. eapply join_well_ordered; eauto.
-      { eapply join_well_ordered; eauto. eapply incr_times_well_ordered. }
-      { eapply singleton_well_ordered. }
+    { exists (times \2/ (fun loc => incr_times) \2/ (fun _ => eq Time.bot)). splits; eauto.
+      { econs 3; eauto. econs; eauto.
+        eapply times_configuration_step_strong_mon; eauto. }
+      { i. eapply join_well_ordered; eauto.
+        { eapply join_well_ordered; eauto. eapply incr_times_well_ordered. }
+        { eapply singleton_well_ordered. }
+      }
+      { i. left. right. eexists. eauto. }
     }
-    { i. left. right. eexists. eauto. }
+    { exists (times \2/ (fun loc => incr_times) \2/ (fun _ => eq Time.bot)). splits; eauto.
+      { econs 3; eauto.
+        { econs. eapply times_configuration_step_strong_mon; eauto. }
+      }
+      { i. eapply join_well_ordered; eauto.
+        { eapply join_well_ordered; eauto. eapply incr_times_well_ordered. }
+        { eapply singleton_well_ordered. }
+      }
+      { i. left. right. eexists. eauto. }
+    }
   }
   { i. exploit IHBEH.
     { eapply Configuration.step_future; eauto. } i. des.
     exploit times_configuration_step_exists; eauto. i. des.
-    exists (times \2/ times0). splits.
-    { econs 4; eauto.
-      { econs. eapply times_configuration_step_strong_mon; eauto. }
-      { eapply le_step_behavior_improve; try apply BEH0.
-        eapply times_configuration_step_strong_all_mon; auto. }
+    { exists (times \2/ times0). splits.
+      { econs 4; eauto.
+        { econs. eapply times_configuration_step_strong_mon; eauto. }
+        { eapply le_step_behavior_improve; try apply BEH0.
+          eapply times_configuration_step_strong_all_mon; auto. }
+      }
+      { i. eapply join_well_ordered; eauto. }
+      { auto. }
+      { auto. }
     }
-    { i. eapply join_well_ordered; eauto. }
-    { auto. }
-    { auto. }
+    { exists (times \2/ times0). splits.
+      { econs 3; eauto.
+        { econs. eapply times_configuration_step_strong_mon; eauto. }
+      }
+      { i. eapply join_well_ordered; eauto. }
+      { auto. }
+      { auto. }
+    }
+  }
+  { i. esplits.
+    { econs 5. }
+    { instantiate (1:=((fun loc => incr_times) \2/ (fun _ => eq Time.bot))).
+      i. eapply join_well_ordered; eauto.
+      { eapply incr_times_well_ordered. }
+      { eapply singleton_well_ordered. }
+    }
+    { i. left. eexists. eauto. }
+    { i. right. auto. }
   }
 Qed.
